permission_bits.v
@@ -89,7 +89,7 @@ Lemma pbits_valid_perm_valid Γ Γm xbs :
   ✓{Γ,Γm}* xbs → Forall sep_valid (tagged_perm <$> xbs).
 Proof. induction 1 as [|?? (?&?&?)]; csimpl; eauto. Qed.
 Lemma pbit_valid_weaken Γ1 Γ2 Γm1 Γm2 xb :
-  ✓ Γ1 → ✓{Γ1,Γm1} xb → Γ1 ⊆ Γ2 → Γm1 ⊆{⇒} Γm2 → ✓{Γ2,Γm2} xb.
+  ✓ Γ1 → ✓{Γ1,Γm1} xb → Γ1 ⊆ Γ2 → Γm1 ⇒ₘ Γm2 → ✓{Γ2,Γm2} xb.
 Proof. intros ? (?&?&?); repeat split; eauto using bit_valid_weaken. Qed.
 Lemma pbit_valid_sep_valid Γ Γm xb  : ✓{Γ,Γm} xb → sep_valid xb.
 Proof. by intros (?&?&?); repeat split. Qed.
@@ -374,8 +374,8 @@ Global Instance:
   PropHolds (✓ Γ) → Transitive (refine Γ meminj_id Γm Γm : relation (pbit Ti)).
 Proof. intros Γ ?????. eapply @pbit_refine_compose; eauto; apply _. Qed.
 Lemma pbit_refine_weaken Γ Γ' f f' Γm1 Γm2 Γm1' Γm2' xb1 xb2 :
-  ✓ Γ → xb1 ⊑{Γ,f@Γm1↦Γm2} xb2 → Γ ⊆ Γ' → Γm1' ⊑{Γ',f'} Γm2' → Γm1 ⊆{⇒} Γm1' →
-  Γm2 ⊆{⇒} Γm2' → meminj_extend f f' Γm1 Γm2 → xb1 ⊑{Γ',f'@Γm1'↦Γm2'} xb2.
+  ✓ Γ → xb1 ⊑{Γ,f@Γm1↦Γm2} xb2 → Γ ⊆ Γ' → Γm1' ⊑{Γ',f'} Γm2' → Γm1 ⇒ₘ Γm1' →
+  Γm2 ⇒ₘ Γm2' → meminj_extend f f' Γm1 Γm2 → xb1 ⊑{Γ',f'@Γm1'↦Γm2'} xb2.
 Proof. intros ? (?&?&[]&[]); repeat split; eauto using bit_refine_weaken. Qed.
 Lemma pbits_refine_perm Γ f Γm1 Γm2 xbs1 xbs2 :
   xbs1 ⊑{Γ,f@Γm1↦Γm2}* xbs2 → tagged_perm <$> xbs1 = tagged_perm <$> xbs2.
